src/tactics.v
@@ -50,7 +50,7 @@ Ltac pack :=
    succeeds? *)
 
 Ltac tc :=
-  eauto 6 with typeclass_instances lia.
+  eauto with typeclass_instances lia.
 
 (* [intuition eauto] can eliminate disjunctions, which is sometimes
    handy. However, it tends to destructure the goal even when it is
